celliocb/CellioAll.v
@@ -1,54 +1,52 @@
 Require Import CRIS Cancel.
 Require Import ImpPrelude.
-Require Import MaincbHeader.
-Require Import 
-  CelliocbHeader CelliocbA CelliocbI MaincbA MaincbI CtxcbHeader CelliocbIAproof MaincbIAproof.
+From CRIS.celliocb Require Import MainHeader CellioHeader CellioA CellioI MainA MainI CtxHeader CellioIAproof MainIAproof.
 
-Section CelliocbAux.
-  Context `{!crisG Γ Σ α β τ Hsub Hinv, _CELL: !celliocbGS}.
+Section CellioAux.
+  Context `{!crisG Γ Σ α β τ Hsub Hinv, _CELL: !cellioGS}.
 
   Variable Ctx : SMod.t.
   Hypothesis ctx_real: SMod.is_real Ctx.
   Hypothesis ctx_mod_wf: Mod.wf (SMod.to_mod ∅ Ctx).
   Hypothesis ctx_cancellable : SMod.cancellable Ctx.
-  Hypothesis ctx_has_foo: fid CtxcbHdr.foo ∈ dom (SMod.fnsems Ctx).
+  Hypothesis ctx_has_foo: fid CtxHdr.foo ∈ dom (SMod.fnsems Ctx).
   Hypothesis ctx_main_disj:
-    ∀ fno, fno ∈ dom (SMod.fnsems Ctx) → fno ∈ dom (Mod.fnsems MaincbI.t) → False.
+    ∀ fno, fno ∈ dom (SMod.fnsems Ctx) → fno ∈ dom (Mod.fnsems MainI.t) → False.
   Hypothesis ctx_cellio_disj:
-    ∀ fno, fno ∈ dom (SMod.fnsems Ctx) → fno ∈ dom (Mod.fnsems CelliocbI.t) → False.
+    ∀ fno, fno ∈ dom (SMod.fnsems Ctx) → fno ∈ dom (Mod.fnsems CellioI.t) → False.
   Hypothesis ctx_main_scope_disj:
-    ∀ mn, mn ∈ (SMod.scopes Ctx) → mn ∈ (Mod.scopes MaincbI.t) → False.
+    ∀ mn, mn ∈ (SMod.scopes Ctx) → mn ∈ (Mod.scopes MainI.t) → False.
   Hypothesis ctx_cellio_scope_disj:
-    ∀ mn, mn ∈ (SMod.scopes Ctx) → mn ∈ (Mod.scopes CelliocbI.t) → False.
+    ∀ mn, mn ∈ (SMod.scopes Ctx) → mn ∈ (Mod.scopes CellioI.t) → False.
 
   Local Definition Ctx_filtered : SMod.t := SMod.filter SFilter.msk_filter_out Ctx.
-  Local Definition mod_top : Mod.t := SMod.to_mod ∅ (SMod.cancel (MaincbA.smod ☆ Ctx_filtered)).
-  Local Definition mod_tgt : Mod.t := MaincbI.t ★ CelliocbI.t ★ (SMod.to_mod ∅ Ctx).
+  Local Definition mod_top : Mod.t := SMod.to_mod ∅ (SMod.cancel (MainA.smod ☆ Ctx_filtered)).
+  Local Definition mod_tgt : Mod.t := MainI.t ★ CellioI.t ★ (SMod.to_mod ∅ Ctx).
 
-  Local Definition sp : specmap := SMod.sp_from (MaincbA.smod ☆ Ctx_filtered).
-  Local Definition mod_src : Mod.t := SMod.to_mod sp MaincbA.smod ★ SMod.to_mod ∅ Ctx.
+  Local Definition sp : specmap := SMod.sp_from (MainA.smod ☆ Ctx_filtered).
+  Local Definition mod_src : Mod.t := SMod.to_mod sp MainA.smod ★ SMod.to_mod ∅ Ctx.
 
   Local Definition init_cond : iProp Σ :=
-    (CelliocbA.init_cond)%I.
+    (CellioA.init_cond)%I.
 
-  Lemma sp_cb: sp.1 !! fid MaincbHdr.input_cb = None.
+  Lemma sp_cb: sp.1 !! fid MainHdr.input_cb = None.
   Proof.
     rewrite lookup_omap !lookup_fmap lookup_omap lookup_union_with.
-    assert (CTXNONE: SMod.fnsems Ctx !! fid MaincbHdr.input_cb = None).
+    assert (CTXNONE: SMod.fnsems Ctx !! fid MainHdr.input_cb = None).
     { eapply not_elem_of_dom. ii. eapply ctx_main_disj; eauto.
-      rewrite /MaincbI.t /MaincbI.smod /SMod.to_mod /= /Mod.fnsems. set_solver.
+      rewrite /MainI.t /MainI.smod /SMod.to_mod /= /Mod.fnsems. set_solver.
     } 
     des. rewrite !lookup_fmap CTXNONE. ss.
   (*SLOW*)Qed.
 
-  Lemma sp_foo: sp.1 !! fid CtxcbHdr.foo = None.
+  Lemma sp_foo: sp.1 !! fid CtxHdr.foo = None.
   Proof.
     rewrite lookup_omap !lookup_fmap lookup_omap lookup_union_with.
-    assert (FIND: exists x, SMod.fnsems Ctx !! fid CtxcbHdr.foo = Some (Some x)).
+    assert (FIND: exists x, SMod.fnsems Ctx !! fid CtxHdr.foo = Some (Some x)).
     { eapply elem_of_dom in ctx_has_foo. inv ctx_has_foo. eauto.
       inv ctx_mod_wf. destruct x; eauto.
-      destruct (SMod.fnsems Ctx !! fid CtxcbHdr.foo) eqn:FIND; ss.
-      inv H. hexploit (wf_fns (fid CtxcbHdr.foo)).
+      destruct (SMod.fnsems Ctx !! fid CtxHdr.foo) eqn:FIND; ss.
+      inv H. hexploit (wf_fns (fid CtxHdr.foo)).
       { rewrite /Mod.fnsems /SMod.to_mod lookup_fmap FIND //. }
       i. ss. inv H.
     }
@@ -59,7 +57,7 @@ Section CelliocbAux.
   Lemma cancel_src:
     refines
       (mod_src, init_cond)
-      (mod_top, init_cond ∗ CelliocbA.cell 0 ∗ Cancel.init_res)%I.
+      (mod_top, init_cond ∗ CellioA.cell 0 ∗ Cancel.init_res)%I.
   Proof.
     etrans.
     { eapply ctxr_refines. ctxr_drop.
@@ -89,15 +87,15 @@ Section CelliocbAux.
     rewrite -SMod.to_mod_cancel_add left_id.
     eapply Cancel.cancellation.
     { apply SMod.cancellable_add.
-      - r; rewrite /= /MaincbA.fnsems //; mod_tac ss.
+      - r; rewrite /= /MainA.fnsems //; mod_tac ss.
       - eapply SFilter.filter_cancellable. et.
     }
     { assert (Ce : SMod.fnsems Ctx !! entry = None).
       { eapply not_elem_of_dom. ii. eapply ctx_main_disj; eauto.
-        rewrite /MaincbI.t /MaincbI.smod /SMod.to_mod /= /Mod.fnsems. set_solver.
+        rewrite /MainI.t /MainI.smod /SMod.to_mod /= /Mod.fnsems. set_solver.
       }
-      assert (Ht : (SMod.sp_from (MaincbA.smod ☆ Ctx_filtered)).1 !! entry =
-        fsp_some MaincbA.main_spec); last (rewrite Ht; clear Ht).
+      assert (Ht : (SMod.sp_from (MainA.smod ☆ Ctx_filtered)).1 !! entry =
+        fsp_some MainA.main_spec); last (rewrite Ht; clear Ht).
       { rewrite /SMod.sp_from /SMod.sp_core_from.
         rewrite !lookup_omap !lookup_fmap lookup_omap lookup_union_with.
         simpl_map; ss. rewrite !lookup_fmap Ce //.
@@ -116,22 +114,22 @@ Section CelliocbAux.
     rewrite /init_cond /mod_src /mod_tgt.
     
     (* solve by transitivity:
-      MaincbI ★ CelliocbI ⊆ MaincbI ★ CelliocbA ⊆ MaincbA ★ CelliocbA 
+      MainI ★ CellioI ⊆ MainI ★ CellioA ⊆ MainA ★ CellioA 
     *)
     etrans.
-    { (* CelliocbI ⊆ctx CelliocbA *)
+    { (* CellioI ⊆ctx CellioA *)
       ctxr_drop. ctxr_rotate. ctxr_drop.
-      eapply main_adequacy, CelliocbIA.sim.
+      eapply main_adequacy, CellioIA.sim.
     }
 
     etrans.
-    { (* MaincbI ★ CelliocbA ⊆ MaincbA *)
+    { (* MainI ★ CellioA ⊆ MainA *)
       ctxr_rotate. ctxr_drop. ctxr_rotate.
-      eapply main_adequacy, MaincbIA.sim; eauto using sp_foo, sp_cb.
+      eapply main_adequacy, MainIA.sim; eauto using sp_foo, sp_cb.
     }
 
     etrans.
-    { (* Ctx ⊆ Ctx *)
+    { (* reorder *)
       ctxr_rotate. ctxr_drop. refl.
     }
 
@@ -142,7 +140,7 @@ Section CelliocbAux.
   Lemma top_tgt :
     refines
       (mod_tgt, emp%I)
-      (mod_top, init_cond ∗ CelliocbA.cell 0 ∗ Cancel.init_res)%I.
+      (mod_top, init_cond ∗ CellioA.cell 0 ∗ Cancel.init_res)%I.
   Proof.
     etrans.
     { eapply src_tgt. }
@@ -151,64 +149,41 @@ Section CelliocbAux.
 
   Lemma tgt_wf: Mod.wf mod_tgt.
   Proof.
-    rewrite /mod_tgt; eapply Mod.add_wf.
-    { econs; eauto; [mod_tac|prove_nodup]. }
-    { eapply Mod.add_wf.
-      { econs; eauto; [mod_tac|prove_nodup]. }
-      { inv ctx_mod_wf. econs.
-        { ii. destruct (SMod.fnsems Ctx !! i) eqn: FIND.
-          { rewrite /Mod.fnsems /SMod.to_mod lookup_fmap FIND /= in H. inv H.
-            destruct o; ss. hexploit (wf_fns i); eauto.
-            rewrite /Mod.fnsems /SMod.to_mod lookup_fmap FIND //.
-          }
-          { rewrite /Mod.fnsems /SMod.to_mod lookup_fmap FIND /= in H. inv H. }
-        }
-        { rewrite /SMod.to_mod /= in wf_scopes. rewrite /SMod.to_mod //. }
-      }
-      { ii. rewrite /Mod.fnsems /SMod.to_mod /= dom_fmap in H0. eauto. }
-      { eapply NoDup_app. esplits; eauto.
-        { prove_nodup. }
-        { inv ctx_mod_wf. rewrite /Mod.scopes /SMod.to_mod /= in wf_scopes.
-          rewrite /Mod.scopes /SMod.to_mod //.
-        }
-      }
+    rewrite /mod_tgt. rewrite !assoc comm.
+    eapply Mod.add_wf; cycle 2; et.
+    { mod_tac. }
+    { eapply NoDup_app. esplits.
+      - apply ctx_mod_wf.
+      - mod_tac.
+      - prove_nodup.
     }
-    { rewrite !Mod.dom_fnsems_add; set_solver. }
-    { eapply NoDup_app. esplits; eauto.
-      { prove_nodup. }
-      { ii. ss. rewrite sorting.merge_sort_Permutation in H0. set_solver. }
-      { ss. rewrite sorting.merge_sort_Permutation.
-        eapply NoDup_cons. esplits; eauto.
-        { ii. eapply ctx_cellio_disj; eauto. set_solver. }
-        { inv ctx_mod_wf. rewrite /Mod.scopes /SMod.to_mod /= in wf_scopes.
-          rewrite /Mod.scopes /SMod.to_mod //.
-        }
-      }
-    }
+    econs.
+    - mod_tac.
+    - prove_nodup.
   (*SLOW*)Qed.
-End CelliocbAux.
+End CellioAux.
 
-Module CelliocbAll.
+Module CellioAll.
   Import inv_instances.
 
-  Local Instance Γ : HRA := ##[invΓ; concΓ; celliocbΓ].
+  Local Instance Γ : HRA := ##[invΓ; concΓ; cellioΓ].
   Local Instance Σ : GRA := ##[Γ; invΣ].
 
   Lemma behavioral_refinement :
-    ∃ β τ (Hinv : invGS Γ Σ α) (_ : crisG Γ Σ α β τ _ Hinv) (_ : celliocbGS),
+    ∃ β τ (Hinv : invGS Γ Σ α) (_ : crisG Γ Σ α β τ _ Hinv) (_ : cellioGS),
     ∀ (Ctx : SMod.t)
       (ctx_real: SMod.is_real Ctx)
       (ctx_mod_wf: Mod.wf (SMod.to_mod ∅ Ctx))
       (ctx_cancellable : SMod.cancellable Ctx)
-      (ctx_has_foo: fid CtxcbHdr.foo ∈ dom (SMod.fnsems Ctx))
+      (ctx_has_foo: fid CtxHdr.foo ∈ dom (SMod.fnsems Ctx))
       (ctx_main_disj:
-        ∀ fno, fno ∈ dom (SMod.fnsems Ctx) → fno ∈ dom (Mod.fnsems MaincbI.t) → False)
+        ∀ fno, fno ∈ dom (SMod.fnsems Ctx) → fno ∈ dom (Mod.fnsems MainI.t) → False)
       (ctx_cellio_disj:
-        ∀ fno, fno ∈ dom (SMod.fnsems Ctx) → fno ∈ dom (Mod.fnsems CelliocbI.t) → False)
+        ∀ fno, fno ∈ dom (SMod.fnsems Ctx) → fno ∈ dom (Mod.fnsems CellioI.t) → False)
       (ctx_main_scope_disj:
-        ∀ mn, mn ∈ (SMod.scopes Ctx) → mn ∈ (Mod.scopes MaincbI.t) → False)
+        ∀ mn, mn ∈ (SMod.scopes Ctx) → mn ∈ (Mod.scopes MainI.t) → False)
       (ctx_cellio_scope_disj:
-        ∀ mn, mn ∈ (SMod.scopes Ctx) → mn ∈ (Mod.scopes CelliocbI.t) → False),
+        ∀ mn, mn ∈ (SMod.scopes Ctx) → mn ∈ (Mod.scopes CellioI.t) → False),
     ∃ src_res tgt_res,
     refines_lmod
       (Mod.to_lmod (mod_tgt Ctx) tgt_res)
@@ -230,6 +205,6 @@ Module CelliocbAll.
     }
     s; i; des; et.
   (*SLOW*)Qed.
-End CelliocbAll.
+End CellioAll.
 
-(* Print Assumptions CelliocbAll.behavioral_refinement. *)
+(* Print Assumptions CellioAll.behavioral_refinement. *)
