celliocb/MainI.v
@@ -1,27 +1,27 @@
 Require Import CRIS.
-Require Import MaincbHeader CelliocbHeader CtxcbHeader.
+From CRIS.celliocb Require Import MainHeader CellioHeader CtxHeader.
 
-Module MaincbI. Section MaincbI.
+Module MainI. Section MainI.
   Context `{!crisG Γ Σ α β τ _S _I}.
 
   Definition scopes : list string := [].
 
   Definition input_cb: Any.t -> itree crisE Any.t :=
     λ _,
-      i <- trigger (@IO _ Z "Input_stdin" tt);;
+      trigger (@IO _ unit "Output_stdout" 42);;;
       i <- trigger (@IO _ Z "Input_db" tt);;
       Ret i↑.
 
   Definition main: Any.t -> itree crisE Any.t :=
     λ _,
-      ccallU (Y:=unit) CelliocbHdr.set MaincbHdr.input_cb;;;
-      trigger (Call CtxcbHdr.foo tt↑);;;
-      x <- ccallU (Y:=Z) CelliocbHdr.get tt;;
+      ccallU (Y:=unit) CellioHdr.set MainHdr.input_cb;;;
+      trigger (Call CtxHdr.foo tt↑);;;
+      x <- ccallU (Y:=Z) CellioHdr.get tt;;
       trigger (@IO _ unit "Print" x);;;
       Ret tt↑.
 
   Definition fnsems : fnsemmap :=
-    {[fid MaincbHdr.input_cb     # ((msk_scp scopes msk_true), (None, input_cb));
+    {[fid MainHdr.input_cb     # ((msk_scp scopes msk_true), (None, input_cb));
       entry  # ((msk_scp scopes msk_true), (None, main))]}.
 
   Program Definition smod: SMod.t := {|
@@ -32,5 +32,5 @@ Module MaincbI. Section MaincbI.
   Solve All Obligations with mod_tac.
   
   Definition t := SMod.to_mod ∅ smod.
-End MaincbI. End MaincbI.
+End MainI. End MainI.
 
