cannon/CannonAll.v
@@ -66,7 +66,7 @@ Section CannonAux.
     eapply Mod.add_wf.
     { econs; eauto; [mod_tac|prove_nodup]. }
     { econs; eauto; [mod_tac|prove_nodup]. }
-    { set_solver. }
+    { mod_tac. }
     { prove_nodup; set_solver. }
   Qed.
 End CannonAux.
