cellio/CellioIAproof.v
@@ -1,5 +1,5 @@
 Require Import CRIS.
-Require Import CellioHeader CellioA CellioI CtxHeader.
+From CRIS.cellio Require Import CellioHeader CellioA CellioI CtxHeader.
 
 Set Implicit Arguments.
 
