cellio/MainA.v
@@ -1,5 +1,5 @@
 Require Import CRIS.
-Require Import CellioA CtxHeader CellioHeader.
+From CRIS.cellio Require Import CellioA CtxHeader CellioHeader.
 
 Set Implicit Arguments.
 
