celliocb/MainHeader.v
@@ -1,7 +1,7 @@
 Require Import CRIS.
 
-Module MaincbHdr.
+Module MainHdr.
   Definition input_stdin : string := "Input_stdin".
   Definition input_db : string := "Input_db".
   Definition input_cb : string := "Input_cb".
-End MaincbHdr.
+End MainHdr.
