celliocb/MainIAproof.v
@@ -1,0 +1,65 @@
+Require Import CRIS.
+From CRIS.celliocb Require Import CellioHeader CellioA MainHeader MainA MainI CtxHeader.
+
+
+Module MainIA. Section MainIA.
+  Import CellioA.
+  Context `{!crisG Γ Σ α β τ _S _I, _CELLIOCB: !cellioGS}.
+
+  Context (sp : specmap).
+  Context (sp_foo: sp.1 !! fid CtxHdr.foo = None).
+  Context (sp_cb: sp.1 !! fid MainHdr.input_cb = None).
+  
+  Local Notation CellioAMod := (CellioA.t).
+  Local Notation MainA := (MainA.t sp).
+  Local Notation IstFull := (IstProd (IstSB MainA.(Mod.scopes) IstTrue) IstEq).
+
+  Lemma simF_cb : ISim.sim_fun open MainA (MainI.t ★ CellioAMod) IstFull (fid MainHdr.input_cb).
+  Proof using.
+    cStartFunSim. unfold MainA.input_cb, MainI.input_cb.
+    cStepsS. cStepsT. cStep. cStep. cStep. iSplit; et.
+  Qed. 
+
+  Lemma simF_main : ISim.sim_fun open MainA (MainI.t ★ CellioAMod) IstFull entry.
+  Proof using sp_foo sp_cb.
+    cStartFunSim.
+    unfold MainA.main, MainI.main.
+    
+    (* Take cell(0) *)
+    cStepsS.
+    iDestruct "ASM" as "[-> ASM]".
+
+    (* Give cell(0) *)
+    cStepsT. cInlineT. cStepsT. cForcesT. iFrame.
+    
+    (* sync callback *)
+    cStepsT. cInlineT. cStepsT. unfold MainI.input_cb.
+    rewrite sp_cb. cInlineS. cStepsS. unfold MainA.input_cb.
+    cStep. cStep. cStepsS. cStepsT. 
+     
+    
+    (* sync foo *)
+    rewrite sp_foo.
+    cCall "IST". iIntros "% % % IST".
+
+    (* TGT : inline get *)
+    cStepsT. cInlineT.
+    cStepsT. unfold get. cForceT ret0.
+    
+    (* TGT : get cell ret *)
+    cForcesT. iFrame.
+
+    cStepsT. cStepsS. 
+    
+    (* sync print *)
+    cStep. cStepsS. cStepsT. cForcesS. iSplit; et. cStep. iFrame; et. 
+  (*SLOW*)Qed.
+
+  Lemma sim : ISim.t open MainA (MainI.t ★ CellioAMod) emp IstFull.
+  Proof using sp_foo sp_cb.
+    cStartModSim.
+    { iIntros "_". unfold IstFull, IstProd. repeat (iExists ∅). ss. }
+    { eapply simF_cb; eauto. }  
+    { eapply simF_main; eauto. }
+  Qed.
+End MainIA. End MainIA.
