promise_free/examples/MPAll.v
@@ -106,10 +106,10 @@ Section MPAux.
     { eapply Mod.add_wf.
       { econs; eauto; [mod_tac|prove_nodup]. }
       { econs; eauto; [mod_tac|prove_nodup]. }
-      { rewrite ?Mod.dom_fnsems_add; set_solver. }
+      { mod_tac. }
       { prove_nodup; set_solver. }
     }
-    { rewrite ?Mod.dom_fnsems_add; set_solver. }
+    { mod_tac. }
     { prove_nodup; set_solver. }
   Qed.
 End MPAux.
